theory/x64Syntax.thy
@@ -217,6 +217,7 @@ datatype instruction =
   | Pimulq_r ireg
   | Pdivl_r ireg
   | Pdivq_r ireg
+  | Pmodq_r ireg
   | Pidivl_r ireg
   | Pidivq_r ireg
 
